% ! TeX root = ..\main.tex

\chapter{Conditional Distributions}

\lecture{10}{Lecture 2}{Wed 1 Dec 2021 10:00}{}

\subsection{Another Deck of Cards}
\begin{eg}
		Draw 2 cards from full deck. Define $Y:$ \# of aces, $X:$ \# of kings (see \autoref{fig:card_table}).
\begin{align*}
		P(\text{one Ace } \mid \text{one King})&=P(Y=1\mid X=1)\\
									&=\frac{P(Y=1, X=1)}{P(X=1)}\\
									&=\frac{f_{X,Y}(1,1)}{f_X(1)}.
\end{align*}
\end{eg}

\subsection{Conditional Mass and Density}
In general,
$$
P(Y=y\mid X=x)=\frac{f_{X,Y}(x,y)}{f_X(x)}.
$$
\begin{definition}
The \textbf{conditional probability mass function} of $Y$ given $X=x$ is
$$
f_{Y|X}(y\mid x)=\frac{f_{X,Y}(x,y)}{f_X(x).}
$$
\end{definition}
Question: Does it sum to 1?
\begin{align*}
    \sum_yf_{Y\mid X}(y\mid X)&=\sum_y\frac{f_{X,Y}(x,y)}{f_X(x)}\\
    &=\frac{1}{f_X(x)}\sum_yf_{X,Y}(x,y)\\
    &=\frac{f_X(x)}{f_X(x)} \\
    &=1. \quad \checkmark
    \end{align*}
\begin{definition}
		The \textbf{conditional cumulative distribution function} of $Y$ given $X=x$ is
$$
F_{Y\mid X}(y\mid x)=\sum_{u\leq y}f_{Y\mid X}(u\mid x)
$$
\end{definition}
\begin{definition}
If $X,Y$ are jointly continuous, we define the \textbf{conditional probability density function} of $Y$ given $X=x$ as
\begin{align*}
f_{Y\mid X}(y\mid x)&=\frac{f_{X,Y}(x,y)}{f_X(x)}.
\end{align*}
\end{definition}

\begin{eg}
Let $X,Y$ be jointly continuous random variables with
$$
f_{X,Y}(x,y)=\begin{cases}8xy, \, &0<x<y<1 \\ 0, \, &\text{otherwise}. \end{cases}
$$
Recall that
$$f_X(x)=4x(1-x^2),\quad  0<x<1.$$
Then
$$
f_{Y\mid X}(y\mid x)=\frac{8xy}{4x(1-x^2)}=\frac{2y}{1-x^2}, \quad x<y<1.
$$
Furthermore,
\begin{align*}
    F_{Y\mid X}(y\mid x)&=\int^y_{-\infty}f_{Y\mid X}(u\mid x) \ du\\
						&=\int^y_x\frac{2u}{1-x^2} \, du\\
    &=\frac{y^2-x^2}{1-x^2}, \quad x<y<1.
\end{align*}
Plug in $y=x$ to check if this is plausible.

\begin{recall}
		$P(A\cap B\cap C)=P(A\mid B\cap C)P(B\mid C)P(C)$. Similarly,
\end{recall}
$$
f_{X,Y}(x,y)=f_{Y\mid X}(y\mid x)f_X(x),
$$
and
$$
f_{X,Y,Z}(x,y,z)=f_{Z\mid X,Y}(z\mid x,y)f_{Y\mid X}(y\mid x)f_X(x).
$$
\end{eg}
\subsubsection{A Simple Model}
\begin{eg}
\begin{center}
$X:$ \# of hurricanes formed, \quad $Y:$ \# of hurricanes making landfall
\end{center}

Suppose that $X\sim$ Poisson($\lambda$) and $(Y\mid X=x)\sim \Bin(x,p).$ Then

$$
f_{X,Y}(x,y)=f_{Y\mid X}(y\mid x)f_X(x)=\binom{x}{y}p^y(1-p)^{x-y}\frac{e^{-\lambda} \lambda^x}{x!}.
$$
supported by $x,y=0,1,2,\ldots,$ $y\leq x.$ Then
\begin{align*}
    f_Y(y)&=\sum_{x}f_{X,Y}{(x,y)}\\
		  &=\sum_{x=y}^\infty\frac{x!}{y!(x-y)!}p^y(1-p)^{x-y}\frac{e^{-\lambda}\lambda x}{x!}\\
		  &=\frac{e^{-\lambda}p^y}{y!}\sum^\infty_{x=y}\frac{(1-p)^{x-y}\lambda^x}{(x-y)!}.
\end{align*}
Let $z=x-y$. Then
\begin{align*}
	f_Y(y)
	&=\frac{e^{-\lambda}p^y}{y!}\lambda^y\sum^\infty_{z=0}\frac{(1-p)^z\lambda^z}{z!}\\
    &=\frac{e^{-\lambda}(\lambda p^y)}{y!} e^{\lambda(1-p)}\\
	&=\frac{e^{-\lambda p}(\lambda p)^y}{y!}\\
    &= \frac{e^{-\lambda p}(\lambda p)^y}{y!},\quad y=0,1,2,\ldots
\end{align*}
This implies that $Y\sim \Poisson(\lambda p)$.
\end{eg}
\vskip.1in
In general, if $X$ is discrete and $Y$ is continuous,
$$
\underbrace{f_{X,Y}(x,y)}_{\text{joint mass / density}}=\underbrace{f_{Y\mid X}(y\mid x)}_{\text{conditional density}}\times\underbrace{f_X(x)}_{\text{marginal mass}}
$$
Moreover,
\[
		\intR \sum_{x}f_{X,Y}(x,y) \, dy=1
.\] 
\subsubsection{Insurance Example}
\begin{eg}
Define
    $Z:$ total value of claims, $Y:$ \# of claims submitted, and $X:$ average \# of claims. Suppose that

    
    $$X\sim \Gamma(\alpha, \lambda), \quad (Y\mid X=x)\sim \Poisson(x).
    $$
    Then
    $$
    (Z\mid Y=y)\sim \text{ some continuous model}.
    $$
\end{eg}
